moving to shallow-embedded predicates: all but spawn

concurrency/semax_conc.v
@@ -542,7 +542,7 @@ Program Definition freelock_spec' cs: funspec := mk_funspec
    | (v, sh, R) =>
      PROP (writable_share sh)
      LOCAL (temp _lock v)
-     SEP (weak_positive_mpred R && emp; lock_inv sh v R; R)
+     SEP (weak_precise_mpred R && weak_positive_mpred R && emp; lock_inv sh v R; R)
    end)
   (fun _ x =>
    match x with
@@ -558,6 +558,9 @@ Next Obligation.
   intro cs; hnf.
   intros.
   destruct x as [[v sh] R]; simpl in *.
+Admitted. (* super_non_expansive obligation of freelock_spec' *)
+(* I added "weak_precise_mpred &&" to freelock's precondition *)
+(*
   apply (nonexpansive_super_non_expansive
    (fun R => (PROP (writable_share sh)
     LOCAL (temp _lock v)
@@ -574,6 +577,7 @@ Next Obligation.
   + apply nonexpansive_lock_inv.
   + apply identity_nonexpansive.
 Qed.
+*)
 Next Obligation.
   intro cs; hnf.
   intros.
@@ -1043,31 +1047,34 @@ Program Definition spawn_spec' := mk_funspec
 Next Obligation.
   hnf; intros.
   destruct x as [[[f b] w] pre]; simpl in *.
-Admitted. (* spawn_spec' Obligation *)
+Admitted. (* super_non_expansive obligation of spawn_spec' *)
 Next Obligation.
   hnf; intros.
   destruct x as [[[f b] w] pre]; simpl in *.
   auto.
 Qed.
 
+Definition gvars := map (fun x => gvar (fst x) (snd x)).
+
 Definition spawn_spec :=
   WITH f : val,
        b : val,
+       globals : list (ident * val),
        PrePost :
          { ty : Type &
           (ty *                     (* WITH clause for spawned function *)
           (ty -> val -> Pred))%type}  (* precondition (postcondition is emp) *)
    PRE [_f OF tptr voidstar_funtype, _args OF tptr tvoid]
      PROP (expr.tc_val (tptr Tvoid) b)
-     LOCAL (temp _args b; temp _f f)
-     SEP
+     (LOCALx (temp _args b :: temp _f f :: gvars globals)
+     (SEP
      (match PrePost with existT ty (_, pre) =>
-      EX _y : ident, EX globals : ty -> list (ident * val),
+      EX _y : ident,
       (func_ptr'
         (WITH y : val, x : ty
           PRE [ _y OF tptr tvoid ]
             PROP ()
-            (LOCALx (temp _y y :: map (fun x => gvar (fst x) (snd x)) (globals x))
+            (LOCALx (temp _y y :: gvars globals)
             (SEP   (Interp (pre x y))))
           POST [tvoid]
             PROP  ()
@@ -1079,7 +1086,7 @@ Definition spawn_spec :=
           existT ty (w, pre) =>
           Interp (pre w b)
       end
-     )
+     )))
    POST [ tvoid  ]
      PROP  ()
      LOCAL ()
@@ -1477,10 +1484,10 @@ Qed.
  *)
 
 Definition concurrent_specs (cs : compspecs) (ext_link : string -> ident) :=
-  (ext_link "acquire"%string, acquire_spec) ::
-  (ext_link "release"%string, release_spec) ::
-  (ext_link "makelock"%string, makelock_spec cs) ::
-  (ext_link "freelock"%string, freelock_spec cs) ::
+  (ext_link "acquire"%string, acquire_spec') ::
+  (ext_link "release"%string, release_spec') ::
+  (ext_link "makelock"%string, makelock_spec' cs) ::
+  (ext_link "freelock"%string, freelock_spec' cs) ::
   (ext_link "spawn"%string, spawn_spec) ::
   nil.
 
